\documentclass[11pt,a4paper]{article}
\usepackage{fullpage}
\usepackage{kpfonts,amsmath,booktabs}

\def\damped{_\text{d}}
\pagestyle{empty}

\begin{document}

\def\dampfactor{\phi_h}
\begin{small}\fontsize{7.5}{10}\rmfamily\tabcolsep=0.1cm
\begin{tabular}{clll} \toprule
{\bf Trend}   & \multicolumn{3}{c}{\bf Seasonal} \\
%\cmidrule{2-4}
& \multicolumn{1}{c}{\bf N} &
\multicolumn{1}{c}{\bf A}
& \multicolumn{1}{c}{\bf M}\\
\cmidrule{2-4}
    & $\hat{y}_{t+h|t} = \ell_t$
    & $\hat{y}_{t+h|t} = \ell_t + s_{t-m+h_m^+}$
    & $\hat{y}_{t+h|t}= \ell_ts_{t-m+h_m^+}$      \\[0.1cm]
{\bf N}
    & $\ell_t = \alpha y_t + (1-\alpha) \ell_{t-1}$
    & $\ell_t = \alpha (y_t - s_{t-m}) + (1-\alpha) \ell_{t-1}$
    & $\ell_t = \alpha (y_t / s_{t-m}) + (1-\alpha) \ell_{t-1}$ \\
    &
    & $s_t = \gamma (y_t - \ell_{t-1}) + (1-\gamma) s_{t-m}$
    & $s_t = \gamma (y_t / \ell_{t-1}) + (1-\gamma) s_{t-m}$                \\
\midrule
    & $\hat{y}_{t+h|t} = \ell_t+hb_t$
    & $\hat{y}_{t+h|t} = \ell_t +hb_t +s_{t-m+h_m^+}$
    & $\hat{y}_{t+h|t}= (\ell_t+hb_t)s_{t-m+h_m^+}$                         \\[0.1cm]
{\bf A}
    & $\ell_t = \alpha y_t + (1-\alpha) (\ell_{t-1}+b_{t-1})$
    & $\ell_t = \alpha (y_t - s_{t-m}) + (1-\alpha)(\ell_{t-1}+b_{t-1})$
    & $\ell_t = \alpha (y_t / s_{t-m}) + (1-\alpha)(\ell_{t-1}+b_{t-1})$    \\

    & $b_t = \beta^* (\ell_t-\ell_{t-1}) + (1-\beta^*) b_{t-1}$
    & $b_t = \beta^* (\ell_t-\ell_{t-1}) + (1-\beta^*) b_{t-1}$
    & $b_t = \beta^* (\ell_t-\ell_{t-1}) + (1-\beta^*) b_{t-1}$             \\
    &
    & $s_t = \gamma (y_t - \ell_{t-1}-b_{t-1}) + (1-\gamma)s_{t-m}$
    & $s_t = \gamma (y_t / (\ell_{t-1}+b_{t-1})) + (1-\gamma)s_{t-m}$\\
\midrule
    & $\hat{y}_{t+h|t} = \ell_t+\dampfactor b_t$
    & $\hat{y}_{t+h|t} = \ell_t+\dampfactor b_t+s_{t-m+h_m^+}$
    & $\hat{y}_{t+h|t}= (\ell_t+\dampfactor b_t)s_{t-m+h_m^+}$ \\[0.1cm]
{\bf A$\damped$ }
    & $\ell_t = \alpha y_t + (1-\alpha) (\ell_{t-1}+\phi b_{t-1})$
    & $\ell_t = \alpha (y_t - s_{t-m}) + (1-\alpha) (\ell_{t-1}+\phi b_{t-1})$
    & $\ell_t = \alpha (y_t / s_{t-m}) + (1-\alpha) (\ell_{t-1}+\phi b_{t-1})$\\
    & $b_t = \beta^* (\ell_t-\ell_{t-1}) + (1-\beta^*) \phi b_{t-1}$
    & $b_t = \beta^* (\ell_t-\ell_{t-1}) + (1-\beta^*) \phi b_{t-1}$
    & $b_t = \beta^* (\ell_t-\ell_{t-1}) + (1-\beta^*) \phi b_{t-1}$\\
    &
    & $s_t = \gamma (y_t - \ell_{t-1}-\phi b_{t-1}) + (1-\gamma)s_{t-m}$
    & $s_t = \gamma (y_t / (\ell_{t-1}+\phi b_{t-1})) + (1-\gamma)s_{t-m}$\\
\bottomrule
\end{tabular}\vspace{0.cm}
\end{small}

\end{document}
